---
title: Derivative & integral table
date: 2022-01-16 19:38:00
description: +C
math: true
categories: 
- Lecture Notes
tags:
- Lecture Notes
- math
---



## Detivative table

$$
\begin{aligned}
	y = c \ \ \ \ &\ \ \ \  y' = 0\\
	y = a^x \ \ \ \ &\ \ \ \ y' = a^x \ln a\\
	y = \log_a x \ \ \ \ &\ \ \ \  y' = \frac{1}{x\ln a}\\
	y = \ln x \ \ \ \ &\ \ \ \ y' = \frac{1}{x}\\
	y = x^a \ \ \ \ &\ \ \ \  y' = ax^{a-1}\\
	y = \sin x    \ \ \ \ &\ \ \ \ y' = \cos x\\
	y = \cos x    \ \ \ \ &\ \ \ \ y' = -\sin x\\
	y = \tan x    \ \ \ \ &\ \ \ \ y' = \sec^2 x\\
	y = \cot x    \ \ \ \ &\ \ \ \ y' = -\csc^2 x\\
	y = \arcsin x \ \ \ \ &\ \ \ \ y' = \frac{1}{\sqrt{1-x^2}}\\
	y = \arccos x \ \ \ \ &\ \ \ \ y' = -\frac{1}{\sqrt{1-x^2}}\\
	y = \arctan x \ \ \ \ &\ \ \ \ y' = \frac{1}{1+x^2}\\
	y = \mathrm{arccot} x \ \ \ \ &\ \ \ \ y' = -\frac{1}{1+x^2}
\end{aligned}
$$

## 积分表

$$
\begin{aligned}
	& \int k\mathrm{d}x = kx\\
	& \int x^a \mathrm{d}x = \frac{1}{a+1} x^{a+1} &(a\neq -1)
	\ \ \\
	& \int \frac{1}{x} \mathrm{d}x = \ln \lvert x\rvert \\
	& \int a^x \mathrm{d}x = \frac{a^x}{\ln a} &(0 < a \neq 1)\\
	& \int e^x \mathrm{d}x = e^x\\
	& \int \sin x \mathrm{d}x = -\cos x \\
	& \int \cos x \mathrm{d}x = \sin x\\
	& \int \sec^2x \mathrm{d}x = \tan x\\
	& \int \csc^2 x\mathrm{d}x = -\cot x \\
	& \int \frac{\mathrm{d}x}{a^2 + x^2} = \frac{1}{a} \arctan \frac{x}{a} & (a\neq 0)\\
	& \int \frac{\mathrm{d}x}{x^2 - a^2} = \frac{1}{2a}\ln \left\lvert \frac{x-a}{x+a} \right\rvert & (a\neq 0)\\
	& \int \frac{\mathrm{d}x}{\sqrt{a^2 - x^2}} = \arcsin \frac{x}{a} & (a>0) \\
	& \int \frac{\mathrm{d}x}{\sqrt{x^2 \pm a^2 }} = \ln \left\lvert x \pm \sqrt{x^2 \pm a^2} \right\rvert
\end{aligned}
$$

## Snippets

$$
\int{e^{ax}}\mathrm{d}x = \frac{1}{a} e^{ax}
$$

## Taylor expansion

$$
f(x) = f(a) + f'(a)(x-a) + \frac{f''(a)}{2!}(x-a)^2 + \frac{f^3(a)}{3!}(x-a)^3 + \cdots + \frac{f^n(a)}{n!}(x-a)^n + \cdots
$$

For example, 

$$
e^{x} = 1 + \frac{x}{1!} + \frac{x^2}{2!} + \frac{x^3}{3!} + \cdots
$$
$$
\cos(x) = 1 - \frac{x^2}{2!} + \frac{x^4}{4!} - \frac{x^6}{6!} + \cdots
$$
$$
\sin(x) = x - \frac{x^3}{3!} + \frac{x^5}{5!} - \frac{x^7}{7!} + \cdots
$$


## 积化和差 和差化积

$$
\begin{aligned}
	sin(\alpha) cos(\beta) 
	&= \frac{
		sin(\alpha + \beta) + sin(\alpha - \beta)
	}{2}\\
	cos(\alpha) sin(\beta) &= \frac{sin(\alpha + \beta) - sin(\alpha - \beta)}{2}\\
	cos(\alpha) cos(\beta) &= \frac{cos(\alpha + \beta) + cos(\alpha - \beta)}{2}\\
	sin(\alpha) sin(\beta) &= - \frac{cos(\alpha + \beta) - cos(\alpha - \beta)}{2}
\end{aligned}
$$

$$
\begin{aligned}
	sin(\alpha) + sin(\beta) &= 2 sin(\frac{\alpha + \beta}{2}) cos(\frac{\alpha - \beta}{2})\\
	sin(\alpha) - sin(\beta) &= 2 cos(\frac{\alpha + \beta}{2}) sin (\frac{\alpha - \beta}{2})\\
	cos(\alpha) + cos(\beta) &= 2 cos(\frac{\alpha + \beta}{2}) cos (\frac{\alpha - \beta}{2})\\
	cos(\alpha) - cos(\beta) &= -2sin(\frac{\alpha + \beta}{2}) sin (\frac{\alpha - \beta}{2})
\end{aligned}
$$
